theory/Dynamic_Semantics.thy
@@ -80,9 +80,6 @@ inductive leaf :: "trace_pool \<Rightarrow> control_path \<Rightarrow> bool" whe
     (\<nexists> pi' . \<not>(trpl pi' = None) \<and> strict_prefix pi pi') \<Longrightarrow> 
     leaf trpl pi"
 
-abbreviation control_path_append :: "control_path => control_label => control_path" (infixl ";;" 61) where
-  "pi;;lab \<equiv> pi @ [lab]"
-
 type_synonym cmmn_set = "(control_path * chan * control_path) set"
 
 inductive concur_step :: "trace_pool * cmmn_set \<Rightarrow> trace_pool * cmmn_set \<Rightarrow> bool" (infix "\<rightarrow>" 55) where 
@@ -92,7 +89,7 @@ inductive concur_step :: "trace_pool * cmmn_set \<Rightarrow> trace_pool * cmmn_
       trpl pi = Some (\<langle>RESULT x; env; \<langle>xk, ek, envk\<rangle> # k\<rangle>) ;
       env x = Some v
     \<rbrakk> \<Longrightarrow>
-    (trpl, ys) \<rightarrow> (trpl(pi;;(LReturn xk) \<mapsto> \<langle>ek; envk(xk \<mapsto> v); k\<rangle>), ys)
+    (trpl, ys) \<rightarrow> (trpl(pi @ [LReturn xk] \<mapsto> \<langle>ek; envk(xk \<mapsto> v); k\<rangle>), ys)
   " |
   Seq_Step: "
     \<lbrakk> 
@@ -100,7 +97,7 @@ inductive concur_step :: "trace_pool * cmmn_set \<Rightarrow> trace_pool * cmmn_
       trpl pi = Some (\<langle>LET x = b in e; env; k\<rangle>) ;
       seq_step (b, env) v
     \<rbrakk> \<Longrightarrow>
-    (trpl, ys) \<rightarrow> (trpl(pi;;(LNext x) \<mapsto> \<langle>e; env(x \<mapsto> v); k\<rangle>), ys)
+    (trpl, ys) \<rightarrow> (trpl(pi @ [LNext x] \<mapsto> \<langle>e; env(x \<mapsto> v); k\<rangle>), ys)
   " |
   Seq_Step_Up: "
     \<lbrakk> 
@@ -108,7 +105,7 @@ inductive concur_step :: "trace_pool * cmmn_set \<Rightarrow> trace_pool * cmmn_
       trpl pi = Some (\<langle>LET x = b in e; env; k\<rangle>) ;
       seq_step_up (b, env) (e', env')
     \<rbrakk> \<Longrightarrow>
-    (trpl, ys) \<rightarrow> (trpl(pi;;(LCall x) \<mapsto> \<langle>e'; env'; \<langle>x, e, env\<rangle> # k\<rangle>), ys)
+    (trpl, ys) \<rightarrow> (trpl(pi @ [LCall x] \<mapsto> \<langle>e'; env'; \<langle>x, e, env\<rangle> # k\<rangle>), ys)
   " |
   Let_Chan: "
     \<lbrakk> 
@@ -116,7 +113,7 @@ inductive concur_step :: "trace_pool * cmmn_set \<Rightarrow> trace_pool * cmmn_
       trpl pi = Some (\<langle>LET x = CHAN \<lparr>\<rparr> in e; env; k\<rangle>)
     \<rbrakk> \<Longrightarrow>
     (trpl, ys) \<rightarrow> (trpl(
-      pi;;(LNext x) \<mapsto> (\<langle>e; env(x \<mapsto> (VChan (Ch pi x))); k\<rangle>)), ys)
+      pi @ [LNext x] \<mapsto> (\<langle>e; env(x \<mapsto> (VChan (Ch pi x))); k\<rangle>)), ys)
   " |
   Let_Spawn: "
     \<lbrakk> 
@@ -124,8 +121,8 @@ inductive concur_step :: "trace_pool * cmmn_set \<Rightarrow> trace_pool * cmmn_
       trpl pi = Some (\<langle>LET x = SPAWN ec in e; env; k\<rangle>)
     \<rbrakk> \<Longrightarrow>
     (trpl, ys) \<rightarrow> (trpl(
-      pi;;(LNext x) \<mapsto> (\<langle>e; env(x \<mapsto> VUnit); k\<rangle>), 
-      pi;;(LSpawn x) \<mapsto> (\<langle>ec; env; []\<rangle>)), ys)
+      pi @ [LNext x] \<mapsto> (\<langle>e; env(x \<mapsto> VUnit); k\<rangle>), 
+      pi @ [LSpawn x] \<mapsto> (\<langle>ec; env; []\<rangle>)), ys)
   " |
   Let_Sync: "
     \<lbrakk>
@@ -145,8 +142,8 @@ inductive concur_step :: "trace_pool * cmmn_set \<Rightarrow> trace_pool * cmmn_
     \<rbrakk> \<Longrightarrow>
     (trpl, ys) \<rightarrow> (
       trpl(
-        pis;;(LNext xs) \<mapsto> (\<langle>es; envs(xs \<mapsto> VUnit); ks\<rangle>), 
-        pir;;(LNext xr) \<mapsto> (\<langle>er; envr(xr \<mapsto> vm); kr\<rangle>)), 
+        pis @ [LNext xs] \<mapsto> (\<langle>es; envs(xs \<mapsto> VUnit); ks\<rangle>), 
+        pir @ [LNext xr] \<mapsto> (\<langle>er; envr(xr \<mapsto> vm); kr\<rangle>)), 
       ys \<union> {(pis, c, pir)})
   "
 
